kalloc/kalloc_kfree_definitions.v
@@ -8,13 +8,19 @@ Require Import VC.kalloc.
 #[export] Instance CompSpecs : compspecs. make_compspecs kalloc.prog. Defined.
 
 (* ================================================================= *)
+(** ** Types and defs *)
+
+Definition PGSIZE : Z := 4096.
+Definition t_run := Tstruct _run noattr.
+Definition t_struct_kmem := Tstruct _struct_kmem noattr.
+
+(* ================================================================= *)
 (** ** Size-based kalloc tokens *)
 
 Definition kalloc_token_sz (sh: share) (n: Z) (p: val) : mpred :=
   !! ((*field_compatible t_run [] p /\*)
       0 < n <= PGSIZE
       /\ malloc_compatible (n) p 
-      /\ malloc_compatible (PGSIZE) p
       /\ writable_share sh
       (*/\  maybe some alignment and physical address checks here *))
   && memory_block sh (n) (p).
@@ -41,7 +47,6 @@ forall  (sh: share) (n: Z) (p: val),
   !! ((*field_compatible t_run [] p /\*)
   0 < n <= PGSIZE
   /\ malloc_compatible (n) p 
-  /\ malloc_compatible (PGSIZE) p
   /\ writable_share sh
   (*/\  maybe some alignment and physical address checks here *))
   && memory_block sh (n) (p).
@@ -55,15 +60,12 @@ Qed.
 (* ================================================================= *)
 (** ** Defining freelistrep *)
 
-Definition PGSIZE : Z := 4096.
-Definition t_run := Tstruct _run noattr.
-Definition t_struct_kmem := Tstruct _struct_kmem noattr.
 
 (* NOTE: assume PGSIZE is greater than sizeof t_run *)
 Fixpoint freelistrep (sh: share) (il: list val) (p: val) : mpred := (* the list contains the next*)
  match il with
  | next::il' =>
-        !! malloc_compatible (PGSIZE) p &&  (* p is compatible with a memory block of size sizeof theader. *)
+        !! malloc_compatible (sizeof t_run) p &&  (* p is compatible with a memory block of size sizeof theader. *)
         (sepcon (data_at sh t_run next p) (* at the location p, there is a t_run structure with the value next *)
         (freelistrep sh il' next) (* "*" ensures no loops... *))
  | nil => !! (p = nullval) && emp
@@ -106,16 +108,7 @@ Ltac refold_freelistrep :=
 Definition Tok_APD := Build_KallocTokenAPD kalloc_token_sz kalloc_token_sz_valid_pointer
   kalloc_token_sz_local_facts.
 
-Definition mem_mgr_internal (gv: globals) (sh : share) (ls: list val) (xx:Z) (original_freelist_pointer:val): mpred := (* I am unsure how to access all these elements.. *)
-    !! (writable_share sh /\
-        is_pointer_or_null original_freelist_pointer /\
-              (((ls = nil) /\ original_freelist_pointer = nullval) \/ 
-              ((ls <> nil) /\ isptr original_freelist_pointer))
-        ) &&
-      (sepcon (data_at sh t_struct_kmem (Vint (Int.repr xx), original_freelist_pointer) (gv _kmem))
-      (freelistrep sh ls original_freelist_pointer)).
-
-Definition mem_mgr_external (gv: globals) : mpred :=
+Definition mem_mgr_impl (gv: globals) : mpred :=
   EX (sh : share), EX (ls: list val), EX (xx:Z), EX (original_freelist_pointer:val), (* I am unsure how to access all these elements.. *)
   !! (writable_share sh /\
     is_pointer_or_null original_freelist_pointer /\
@@ -125,34 +118,8 @@ Definition mem_mgr_external (gv: globals) : mpred :=
   (sepcon (data_at sh t_struct_kmem (Vint (Int.repr xx), original_freelist_pointer) (gv _kmem))
   (freelistrep sh ls original_freelist_pointer)).
 
-Lemma mem_mgr_internal_entails_mem_mgr_external :
-  forall gv sh ls xx original_freelist_pointer,
-    mem_mgr_internal gv sh ls xx original_freelist_pointer
-    |-- mem_mgr_external gv.
-Proof.
-  intros gv sh ls xx original_freelist_pointer.
-  unfold mem_mgr_internal.
-  unfold mem_mgr_external.
-  Intros.
-  Exists sh ls xx original_freelist_pointer.
-  entailer!.
-Qed.
 
-Lemma mem_mgr_local_facts :
-  forall gv,
-    (mem_mgr_external gv) |-- (EX (sh : share), EX (ls : list val), EX (original_freelist_pointer : val),
-      !! (writable_share sh /\
-          is_pointer_or_null original_freelist_pointer /\
-          (((ls = nil) /\ original_freelist_pointer = nullval) \/ 
-           ((ls <> nil) /\ isptr original_freelist_pointer)))).
-Proof.
-  intros. unfold mem_mgr_external. Intros sh ls xx original_freelist_pointer.
-  Exists sh ls original_freelist_pointer.
-  entailer!.
-Qed.
-
-
-Definition KF_APD := Build_KallocFreeAPD Tok_APD mem_mgr_external mem_mgr_local_facts.
+Definition KF_APD := Build_KallocFreeAPD Tok_APD mem_mgr_impl.
 
 (* ================================================================= *)
 (** ** Constructing Vprog and Gprog *)
@@ -165,45 +132,6 @@ Definition KF_globals_external gv : mpred:= ASI_kalloc.mem_mgr KF_APD gv.
 Definition KFVprog : varspecs. mk_varspecs kalloc.prog. Defined.
 Definition KFGprog: funspecs := KF_imported_specs ++ KF_internal_specs.
 
-(* ================================================================= *)
-(** ** Lemma to unfold mem_mgr *)
-
-Lemma mem_mgr_internal_split: 
- forall (gv:globals) (sh:share) (ls: list val) (xx:Z) (original_freelist_pointer:val),
-  mem_mgr_internal gv sh ls xx original_freelist_pointer
-  = 
-  !! (writable_share sh /\
-        is_pointer_or_null original_freelist_pointer /\
-              (((ls = nil) /\ original_freelist_pointer = nullval) \/ 
-              ((ls <> nil) /\ isptr original_freelist_pointer))
-        ) &&
-      (sepcon (data_at sh t_struct_kmem (Vint (Int.repr xx), original_freelist_pointer) (gv _kmem))
-      (freelistrep sh ls original_freelist_pointer)).
-Proof.
-  intros. apply pred_ext.
-  - unfold mem_mgr_internal. entailer!.
-  - unfold mem_mgr_internal. entailer!.
-Qed.
-
-Lemma mem_mgr_external_split: 
- forall (gv:globals),
-  mem_mgr_external gv 
-  = 
-  EX (sh : share), EX (ls: list val), EX (xx:Z), EX (original_freelist_pointer:val),
-  !! (writable_share sh /\
-        is_pointer_or_null original_freelist_pointer /\
-              (((ls = nil) /\ original_freelist_pointer = nullval) \/ 
-              ((ls <> nil) /\ isptr original_freelist_pointer))
-        ) &&
-      (sepcon (data_at sh t_struct_kmem (Vint (Int.repr xx), original_freelist_pointer) (gv _kmem))
-      (freelistrep sh ls original_freelist_pointer)).
-Proof.
-  intros. apply pred_ext.
-  - unfold mem_mgr_external. entailer!.
-  Exists sh ls xx original_freelist_pointer. entailer!.
-  - unfold mem_mgr_external. entailer!.
-  Exists sh ls xx original_freelist_pointer. entailer!.
-Qed.
 
 
 (*************************)
